## ?q1 
$$(LL\top)_{ii} = \sum_{k=1}^{i}L_{ik}^2$$
$$
C = AB
$$
$$
C_{ij} = \sum_k A_{ik} \times B_{kj}
$$
$$
C = LL^T \quad A = L \quad B = L^T
$$
$$
C_{ij} = (LL^T)_{ij} = \sum_k L_{ik} \times L^T_{kj}
$$
$$
L^T_{kj} = L_{jk} \quad (LL^T)_{ij} = \sum_k L_{ik} \times L_{jk}
$$
$$
(LL^T)_{ii} \quad j = i \quad (LL^T)_{ii} = \sum_k L_{ik} \times L_{ik} = \sum_k (L_{ik})^2
$$
$$ 
\sum_{k=1}^{n} (L_{ik})^2 = \sum_{k=1}^{i} (L_{ik})^2 + \sum_{k=i+1}^{n} (L_{ik})^2 = \sum_{k=1}^{i} (L_{ik})^2 + 0
$$
$$
(LL^T)_{ii} = \sum_{k=1}^{i} (L_{ik})^2
$$

## ?q2
$$\det \Sigma = \prod_{k=1}^{d}\lambda_k$$
$$p(\lambda) = \det(\Sigma - \lambda I)$$
$$\lambda_1 ,\lambda_2 ,\lambda_3 \cdots \lambda_d$$
$$p(\lambda) = (\lambda_1 - \lambda)(\lambda_2 - \lambda) \cdots (\lambda_d - \lambda) = \prod_{k=1}^{d} \lambda_k - \lambda$$
$$/lambda = 0 \Rightarrow \det(\Sigma - 0\ast I) = \prod_{k=1}^{d} \lambda_k$$